SSA/Experimental/Bits/Fast/Tests.lean
@@ -70,7 +70,7 @@ example (w : Nat) (a b : BitVec w) : (a + b = b + a)  := by
   bv_automata_gen (config := {backend := .circuit_cadical_verified} )
 
 example (w : Nat) (a : BitVec w) : (a = a + 0#w) ∨ (a = a - a)  := by
-  fail_if_success bv_automata_gen (config := {backend := .circuit_cadical_verified 20 } )
+  bv_automata_gen (config := {backend := .circuit_cadical_verified 20 } )
   fail_if_success bv_automata_gen (config := {backend := .circuit_cadical_unverified 20 } )
   sorry
 
